Definition of sim_term/sim_value and proof of reflexivity (modulo strong induction principle)

theories/syntax.v
@@ -282,3 +282,278 @@ Hint Rewrite
   fv_Value_eq
   fv_Fold_eq
   : fv.
+
+Import List.ListNotations.
+Require Import Autosubst_FreeVars.
+Open Scope list.
+  
+Definition subst_of_env sigma :=
+  fun n =>
+  match List.nth_error sigma n with
+  | None => ids (n - List.length sigma)
+  | Some t => Value t
+  end
+.
+
+Notation "'soe' sigma n" := (
+match List.nth_error sigma n with
+| None => ids (n - List.length sigma)
+| Some t => Value t
+end)
+(at level 69, sigma at level 1, n at level 1).
+
+Theorem soe_nil:
+  subst_of_env [] = ids.
+Proof.
+  eapply FunctionalExtensionality.functional_extensionality.
+  induction x; eauto.
+Qed.
+
+Lemma soe_cons v sigma:
+  subst_of_env (v :: sigma) = (Value v) .: subst_of_env sigma.
+Proof.
+  eapply FunctionalExtensionality.functional_extensionality.
+  induction x; asimpl; eauto.
+Qed.
+
+Theorem subst_env_regular:
+  forall sigma: list value,
+  regular (subst_of_env sigma).
+Proof.
+  intros.
+  exists (List.length sigma), 0.
+  eapply FunctionalExtensionality.functional_extensionality.
+  unfold subst_of_env; intros; asimpl.
+  destruct (List.nth_error_None sigma (List.length sigma + x)) as [_ H].
+  rewrite H.
+  f_equal.
+  all: lia.
+Qed.
+
+Lemma subst_env_0: forall t v, t.[subst_of_env [v]] = t.[Value v/].
+Proof.
+  intros.
+  repeat progress (
+    try rewrite soe_nil;
+    try rewrite soe_cons;
+    try reflexivity).
+Qed.
+
+Lemma subst_env_fv_sub:
+  forall sigma t k,
+    fv k t ->
+    fv (k-List.length sigma) (t.[subst_of_env sigma]).
+Proof.
+  induction sigma.
+  * rewrite soe_nil.
+    intros; asimpl.
+    replace (k - 0) with k.
+    all: eauto; lia.
+  * rewrite soe_cons.
+    intros.
+    asimpl.
+    replace t.[Value a .: subst_of_env sigma] with (t.[Value a/].[subst_of_env sigma]) by autosubst.
+    replace (k - S (List.length sigma)) with (pred k - (List.length sigma)) by lia.
+    eapply IHsigma.
+    { induction k; asimpl; eauto.
+      { replace 0 with (0 - 1) by lia.
+        eapply fv_closed_kregular_subst; eauto.
+        { induction x; asimpl; unfold closed; fv; lia. }
+      }
+      { replace k with (S k - 1) by lia.
+        eapply fv_closed_kregular_subst; eauto.
+        { induction x; asimpl; unfold closed; fv; lia. }
+      }
+    }
+Qed.
+
+Lemma subst_env_fv_closed:
+  forall sigma t,
+    fv (List.length sigma) t ->
+    closed (t.[subst_of_env sigma]).
+Proof.
+  unfold closed.
+  intros.
+  replace 0 with (List.length sigma - List.length sigma) by lia.
+  eapply subst_env_fv_sub.
+  eauto.
+Qed.
+
+(* Strong induction princple for terms and values *)
+
+Theorem term_value_ind
+  : forall (P : term -> Prop) (P0 : value -> Prop),
+      (forall x : var, P (Var x)) ->
+      (forall t1 : term, P t1 -> forall t2 : term, P t2 -> P (App t1 t2)) ->
+      (forall t : {bind term}, P t -> P (Lam t)) ->
+      (forall arg : term, P arg -> P (ErrorOnEmpty arg)) ->
+      (forall arg : term, P arg -> P (DefaultPure arg)) ->
+      (forall (ts : list term), List.Forall P ts -> forall (tj : term),
+       P tj -> forall tc : term, P tc -> P (Default ts tj tc)) ->
+      P Empty ->
+      P Conflict ->
+      (forall v : value, P0 v -> P (Value v)) ->
+      (forall x : string, P (FreeVar x)) ->
+      (forall (op : op) (t1 : term),
+       P t1 -> forall t2 : term, P t2 -> P (Binop op t1 t2)) ->
+      (forall u : term,
+       P u ->
+       forall t1 : term,
+       P t1 -> forall t2 : {bind term}, P t2 -> P (Match_ u t1 t2)) ->
+      P ENone ->
+      (forall t : term, P t -> P (ESome t)) ->
+      (forall f : term,
+       P f -> forall (ts : list term), List.Forall P ts -> forall (t : term), P t -> P (Fold f ts t)) ->
+      (forall t : term,
+       P t ->
+       forall ta : term, P ta -> forall tb : term, P tb -> P (If t ta tb)) ->
+      (forall b : bool, P0 (Bool b)) ->
+      (forall i : Z, P0 (Int i)) ->
+      (forall t : {bind term},
+       P t -> forall sigma : list value, List.Forall P0 sigma -> P0 (Closure t sigma)) ->
+      P0 VNone ->
+      P0 VUnit ->
+      (forall v : value, P0 v -> P0 (VSome v)) ->
+      (forall v : value, P0 v -> P0 (VPure v)) ->
+      (forall t : term, P t) /\ (forall v : value, P0 v).
+Admitted.
+
+
+Inductive sim_term : term -> term -> Prop :=
+  | sim_term_var : forall x y, x = y -> sim_term (Var x) (Var y)
+  | sim_term_app : forall t1 t2 u1 u2,
+      sim_term t1 u1 ->
+      sim_term t2 u2 ->
+      sim_term (App t1 t2) (App u1 u2)
+  | sim_term_lam : forall t1 u1,
+      sim_term t1 u1 ->
+      sim_term (Lam t1) (Lam u1)
+  | sim_term_value : forall v1 w1,
+      sim_value v1 w1 ->
+      sim_term (Value v1) (Value w1)
+  | sim_term_erroronempty : forall t1 t2,
+      sim_term t1 t2 ->
+      sim_term (ErrorOnEmpty t1) (ErrorOnEmpty t2)
+  | sim_term_defaultpure : forall t1 t2,
+      sim_term t1 t2 ->
+      sim_term (DefaultPure t1) (DefaultPure t2)
+  | sim_term_default : forall ts1 ts2 tj1 tj2 tc1 tc2,
+      List.Forall2 sim_term ts1 ts2 ->
+      sim_term tj1 tj2 ->
+      sim_term tc1 tc2 ->
+      sim_term (Default ts1 tj1 tc1) (Default ts2 tj2 tc2)
+  | sim_term_empty : sim_term Empty Empty
+  | sim_term_conflict : sim_term Conflict Conflict
+  | sim_term_freevar : forall x y, x = y -> sim_term (FreeVar x) (FreeVar y)
+  | sim_term_binop : forall op1 op2 t1 t2 u1 u2,
+      op1 = op2 ->
+      sim_term t1 u1 ->
+      sim_term t2 u2 ->
+      sim_term (Binop op1 t1 t2) (Binop op2 u1 u2)
+  | sim_term_match : forall u1 u2 t1 t2 t3 t4,
+      sim_term u1 u2 ->
+      sim_term t1 t2 ->
+      sim_term t3 t4 ->
+      sim_term (Match_ u1 t1 t3) (Match_ u2 t2 t4)
+  | sim_term_enone : sim_term ENone ENone
+  | sim_term_esome : forall t1 t2,
+      sim_term t1 t2 ->
+      sim_term (ESome t1) (ESome t2)
+  | sim_term_fold : forall f1 f2 ts1 ts2 t1 t2,
+      sim_term f1 f2 ->
+      List.Forall2 sim_term ts1 ts2 ->
+      sim_term t1 t2 ->
+      sim_term (Fold f1 ts1 t1) (Fold f2 ts2 t2)
+  | sim_term_if : forall t1 t2 ta1 ta2 tb1 tb2,
+      sim_term t1 t2 ->
+      sim_term ta1 ta2 ->
+      sim_term tb1 tb2 ->
+      sim_term (If t1 ta1 tb1) (If t2 ta2 tb2)
+
+with sim_value : value -> value -> Prop :=
+  | sim_value_bool : forall b1 b2,
+      b1 = b2 ->
+      sim_value (Bool b1) (Bool b2)
+  | sim_value_int : forall i1 i2,
+      i1 = i2 ->
+      sim_value (Int i1) (Int i2)
+  | sim_value_closure : forall t1 t2 sigma1 sigma2,
+      sim_term t1.[up (subst_of_env sigma1)] t2.[up (subst_of_env sigma2)] ->
+      sim_value (Closure t1 sigma1) (Closure t2 sigma2)
+  | sim_value_vnone : sim_value VNone VNone
+  | sim_value_vunit : sim_value VUnit VUnit
+  | sim_value_vsome : forall v1 v2,
+      sim_value v1 v2 ->
+      sim_value (VSome v1) (VSome v2)
+  | sim_value_vpure : forall v1 v2,
+      sim_value v1 v2 ->
+      sim_value (VPure v1) (VPure v2).
+
+Require Import Coq.Classes.SetoidClass.
+
+Lemma sim_term_ren:
+  forall t1 t2,
+    sim_term t1 t2 ->
+    forall xi,
+      sim_term t1.[ren xi] t2.[ren xi].
+Proof.
+  induction 1; intros; subst; asimpl.
+  all: try econstructor; eauto.
+  { induction H; simpl; econstructor; eauto. admit "need stronger induction priple". }
+  { induction H0; simpl; econstructor; eauto. admit "need stronger induction priple". }
+Admitted.
+
+Lemma sim_term_subst:
+  forall t1 t2,
+    sim_term t1 t2 ->
+    forall sigma1 sigma2,
+      (forall x, sim_term (sigma1 x) (sigma2 x)) ->
+      sim_term t1.[sigma1] t2.[sigma2].
+Proof.
+  induction 1; intros; subst; asimpl.
+  all: try econstructor; eauto.
+  { eapply IHsim_term.
+    induction x; asimpl.
+    { econstructor; eauto. }
+    { eapply sim_term_ren; eauto. }
+  }
+  { induction H; asimpl; econstructor; eauto. admit "need stronger induction priple". }
+  { eapply IHsim_term3.
+    induction x; asimpl.
+    { econstructor; eauto. }
+    { eapply sim_term_ren; eauto. }
+  }
+  { induction H0; asimpl; econstructor; eauto. admit "need stronger induction priple". }
+Admitted.
+
+
+Lemma sim_term_refl: Reflexive sim_term /\ Reflexive sim_value.
+Proof.
+  eapply term_value_ind; intros.
+  all: try (econstructor; eauto).
+  { induction H; econstructor; eauto. }
+  { induction H0; econstructor; eauto. }
+  {
+    eapply sim_term_subst.
+    { eauto. }
+    { intro x; case x; asimpl.
+      { econstructor; eauto. }
+      { intros; eapply sim_term_ren.
+        revert n.
+        induction sigma.
+        { rewrite soe_nil; econstructor; eauto. }
+        { inversion H0; subst; intros. case n; asimpl.
+          { econstructor; eauto. }
+          { intros. rewrite soe_cons.
+            eapply IHsigma; eauto.
+          }
+        }
+      }
+    }
+  }
+Qed.
+
+
+Instance Reflexive_sim_term : Reflexive sim_term. eapply sim_term_refl. Qed. 
+Instance Symmetric_sim_term : Symmetric sim_term. Admitted.
+Instance Transtive_sim_term : Transitive sim_term. Admitted.
